- Recognize __builtin_fabs as an operator, not just a builtin,   enabling more aggressive optimizations. - Less aggressive CSE for EF_builtin builtins, causes problems   for __builtin_write{16,32}_reversed.
git-svn-id: https://yquem.inria.fr/compcert/svn/compcert/trunk@2363 fca1b0fc-160b-0410-b1d3-a4f43f01ea2e

cfrontend/C2C.ml
@@ -576,6 +576,9 @@ let rec convertExpr env e =
  | C.ECall({edesc = C.EVar {name = "__builtin_memcpy_aligned"}}, args) ->
       make_builtin_memcpy (convertExprList env args)
 
+  | C.ECall({edesc = C.EVar {name = "__builtin_fabs"}}, [arg]) ->
+      Eunop(Oabsfloat, convertExpr env arg, ty)
+
   | C.ECall(fn, args) ->
       if not (supported_return_type env e.etyp) then
         unsupported ("function returning a result of type " ^ string_of_type e.etyp);
